\documentclass[10pt,fleqn]{article}
% \usepackage[journal=rsc]{chemstyle}
% \usepackage{mhchem}
\usepackage{amsmath}
\usepackage{amssymb}
\usepackage{amsfonts}
\usepackage{esint}
\usepackage{bbm}
\usepackage{amscd}
\usepackage{picinpar}
\usepackage{graphicx}
\usepackage{tikz}
\usepackage{tikz-3dplot}
\usepackage{indentfirst}
\usepackage{wrapfig}
\usepackage{units}
\usepackage{textcomp}
\usepackage[utf8x]{inputenc}
% \usepackage{feyn}
\usepackage{feynmp}
\usepackage{xkeyval}
\usepackage{xargs}
\usepackage{verbatim}
\usepackage{pgfplots}
\usepackage{hyperref}
\usetikzlibrary{
  arrows,
  calc,
  decorations.pathmorphing,
  decorations.pathreplacing,
  decorations.markings,
  fadings,
  positioning,
  shapes
}

\DeclareGraphicsRule{*}{mps}{*}{}
\newcommand{\ud}{\mathrm{d}}
\newcommand{\ue}{\mathrm{e}}
\newcommand{\ui}{\mathrm{i}}
\newcommand{\res}{\mathrm{Res}}
\newcommand{\Tr}{\mathrm{Tr}}
\newcommand{\dsum}{\displaystyle\sum}
\newcommand{\dprod}{\displaystyle\prod}
\newcommand{\dlim}{\displaystyle\lim}
\newcommand{\dint}{\displaystyle\int}
\newcommand{\fsno}[1]{{\!\not\!{#1}}}
\newcommand{\eqar}[1]
{
  \begin{align*}
    #1
  \end{align*}
}
\newcommand{\texp}[2]{\ensuremath{{#1}\times10^{#2}}}
\newcommand{\dexp}[2]{\ensuremath{{#1}\cdot10^{#2}}}
\newcommand{\eval}[2]{{\left.{#1}\right|_{#2}}}
\newcommand{\paren}[1]{{\left({#1}\right)}}
\newcommand{\lparen}[1]{{\left({#1}\right.}}
\newcommand{\rparen}[1]{{\left.{#1}\right)}}
\newcommand{\abs}[1]{{\left|{#1}\right|}}
\newcommand{\sqr}[1]{{\left[{#1}\right]}}
\newcommand{\crly}[1]{{\left\{{#1}\right\}}}
\newcommand{\angl}[1]{{\left\langle{#1}\right\rangle}}
\newcommand{\tpdiff}[4][{}]{{\paren{\frac{\partial^{#1} {#2}}{\partial {#3}{}^{#1}}}_{#4}}}
\newcommand{\tpsdiff}[4][{}]{{\paren{\frac{\partial^{#1}}{\partial {#3}{}^{#1}}{#2}}_{#4}}}
\newcommand{\pdiff}[3][{}]{{\frac{\partial^{#1} {#2}}{\partial {#3}{}^{#1}}}}
\newcommand{\diff}[3][{}]{{\frac{\ud^{#1} {#2}}{\ud {#3}{}^{#1}}}}
\newcommand{\psdiff}[3][{}]{{\frac{\partial^{#1}}{\partial {#3}{}^{#1}} {#2}}}
\newcommand{\sdiff}[3][{}]{{\frac{\ud^{#1}}{\ud {#3}{}^{#1}} {#2}}}
\newcommand{\tpddiff}[4][{}]{{\left(\dfrac{\partial^{#1} {#2}}{\partial {#3}{}^{#1}}\right)_{#4}}}
\newcommand{\tpsddiff}[4][{}]{{\paren{\dfrac{\partial^{#1}}{\partial {#3}{}^{#1}}{#2}}_{#4}}}
\newcommand{\pddiff}[3][{}]{{\dfrac{\partial^{#1} {#2}}{\partial {#3}{}^{#1}}}}
\newcommand{\ddiff}[3][{}]{{\dfrac{\ud^{#1} {#2}}{\ud {#3}{}^{#1}}}}
\newcommand{\psddiff}[3][{}]{{\frac{\partial^{#1}}{\partial{}^{#1} {#3}} {#2}}}
\newcommand{\sddiff}[3][{}]{{\frac{\ud^{#1}}{\ud {#3}{}^{#1}} {#2}}}
\usepackage{fancyhdr}
\usepackage{multirow}
\usepackage{fontenc}
% \usepackage{tipa}
\usepackage{ulem}
\usepackage{color}
\usepackage{cancel}
\newcommand{\hcancel}[2][black]{\setbox0=\hbox{#2}%
  \rlap{\raisebox{.45\ht0}{\textcolor{#1}{\rule{\wd0}{1pt}}}}#2}
\pagestyle{fancy}
\setlength{\headheight}{67pt}
\fancyhead{}
\fancyfoot{}
\fancyfoot[C]{\thepage}
\fancyhead[R]{}
\renewcommand{\footruleskip}{0pt}
\renewcommand{\headrulewidth}{0.4pt}
\renewcommand{\footrulewidth}{0pt}

\newcommand\pgfmathsinandcos[3]{%
  \pgfmathsetmacro#1{sin(#3)}%
  \pgfmathsetmacro#2{cos(#3)}%
}
\newcommand\LongitudePlane[3][current plane]{%
  \pgfmathsinandcos\sinEl\cosEl{#2} % elevation
  \pgfmathsinandcos\sint\cost{#3} % azimuth
  \tikzset{#1/.estyle={cm={\cost,\sint*\sinEl,0,\cosEl,(0,0)}}}
}
\newcommand\LatitudePlane[3][current plane]{%
  \pgfmathsinandcos\sinEl\cosEl{#2} % elevation
  \pgfmathsinandcos\sint\cost{#3} % latitude
  \pgfmathsetmacro\yshift{\cosEl*\sint}
  \tikzset{#1/.estyle={cm={\cost,0,0,\cost*\sinEl,(0,\yshift)}}} %
}
\newcommand\DrawLongitudeCircle[2][1]{
  \LongitudePlane{\angEl}{#2}
  \tikzset{current plane/.prefix style={scale=#1}}
  % angle of "visibility"
  \pgfmathsetmacro\angVis{atan(sin(#2)*cos(\angEl)/sin(\angEl))} %
  \draw[current plane] (\angVis:1) arc (\angVis:\angVis+180:1);
  \draw[current plane,dashed] (\angVis-180:1) arc (\angVis-180:\angVis:1);
}
\newcommand\DrawLatitudeCircleArrow[2][1]{
  \LatitudePlane{\angEl}{#2}
  \tikzset{current plane/.prefix style={scale=#1}}
  \pgfmathsetmacro\sinVis{sin(#2)/cos(#2)*sin(\angEl)/cos(\angEl)}
  % angle of "visibility"
  \pgfmathsetmacro\angVis{asin(min(1,max(\sinVis,-1)))}
  \draw[current plane,decoration={markings, mark=at position 0.6 with {\arrow{<}}},postaction={decorate},line width=.6mm] (\angVis:1) arc (\angVis:-\angVis-180:1);
  \draw[current plane,dashed,line width=.6mm] (180-\angVis:1) arc (180-\angVis:\angVis:1);
}
\newcommand\DrawLatitudeCircle[2][1]{
  \LatitudePlane{\angEl}{#2}
  \tikzset{current plane/.prefix style={scale=#1}}
  \pgfmathsetmacro\sinVis{sin(#2)/cos(#2)*sin(\angEl)/cos(\angEl)}
  % angle of "visibility"
  \pgfmathsetmacro\angVis{asin(min(1,max(\sinVis,-1)))}
  \draw[current plane] (\angVis:1) arc (\angVis:-\angVis-180:1);
  \draw[current plane,dashed] (180-\angVis:1) arc (180-\angVis:\angVis:1);
}
\newcommand\coil[1]{
  {\rh * cos(\t * pi r)}, {\apart * (2 * #1 + \t) + \rv * sin(\t * pi r)}
}
\makeatletter
\define@key{DrawFromCenter}{style}[{->}]{
  \tikzset{DrawFromCenterPlane/.style={#1}}
}
\define@key{DrawFromCenter}{r}[1]{
  \def\@R{#1}
}
\define@key{DrawFromCenter}{center}[(0, 0)]{
  \def\@Center{#1}
}
\define@key{DrawFromCenter}{theta}[0]{
  \def\@Theta{#1}
}
\define@key{DrawFromCenter}{phi}[0]{
  \def\@Phi{#1}
}
\presetkeys{DrawFromCenter}{style, r, center, theta, phi}{}
\newcommand*\DrawFromCenter[1][]{
  \setkeys{DrawFromCenter}{#1}{
    \pgfmathsinandcos\sint\cost{\@Theta}
    \pgfmathsinandcos\sinp\cosp{\@Phi}
    \pgfmathsinandcos\sinA\cosA{\angEl}
    \pgfmathsetmacro\DX{\@R*\cost*\cosp}
    \pgfmathsetmacro\DY{\@R*(\cost*\sinp*\sinA+\sint*\cosA)}
    \draw[DrawFromCenterPlane] \@Center -- ++(\DX, \DY);
  }
}
\newcommand*\DrawFromCenterText[2][]{
  \setkeys{DrawFromCenter}{#1}{
    \pgfmathsinandcos\sint\cost{\@Theta}
    \pgfmathsinandcos\sinp\cosp{\@Phi}
    \pgfmathsinandcos\sinA\cosA{\angEl}
    \pgfmathsetmacro\DX{\@R*\cost*\cosp}
    \pgfmathsetmacro\DY{\@R*(\cost*\sinp*\sinA+\sint*\cosA)}
    \draw[DrawFromCenterPlane] \@Center -- ++(\DX, \DY) node {#2};
  }
}
\makeatother
\tikzstyle{snakearrow} = [decorate, decoration={pre length=0.2cm,
  post length=0.2cm, snake, amplitude=.4mm,
  segment length=2mm},thick, ->]
%% document-wide tikz options and styles
\tikzset{%
  >=latex, % option for nice arrows
  inner sep=0pt,%
  outer sep=2pt,%
  mark coordinate/.style={inner sep=0pt,outer sep=0pt,minimum size=3pt,
    fill=black,circle}%
}
\addtolength{\hoffset}{-1.3cm}
\addtolength{\voffset}{-2cm}
\addtolength{\textwidth}{3cm}
\addtolength{\textheight}{2.5cm}
\renewcommand{\footskip}{10pt}
\setlength{\headwidth}{\textwidth}
\setlength{\headsep}{20pt}
\setlength{\marginparwidth}{0pt}
\parindent=0pt
\title{Exact solutions for 2x2 master equation}
\begin{document}

\maketitle

\section{Master equation}
Master equation for a driven two level system
\eqar{
  \diff{\rho}{t}=&-\ui\sqr{H, \rho}+\sum_m C_m\rho C^\dagger_m-\frac12\sum_m\paren{C^\dagger_m C_m\rho+\rho C^\dagger_m C_m}\\
  H=&\frac12\begin{pmatrix}
    0&-\ui\Omega\\
    \ui\Omega&0
  \end{pmatrix}\\
  \rho=&\begin{pmatrix}
    \rho_{11}&\rho_{12}\\
    \rho_{21}&\rho_{22}
  \end{pmatrix}\\
}

\section{Non-state changing decay}
Jump operators
\eqar{
  C_1=&\sqrt{\Gamma}\begin{pmatrix}
    1&0\\
    0&0
  \end{pmatrix}\\
  C_2=&\sqrt{\Gamma}\begin{pmatrix}
    0&0\\
    0&1
  \end{pmatrix}\\
  C^\dagger_1=&\sqrt{\Gamma}\begin{pmatrix}
    1&0\\
    0&0
  \end{pmatrix}\\
  C^\dagger_2=&\sqrt{\Gamma}\begin{pmatrix}
    0&0\\
    0&1
  \end{pmatrix}\\
  C^\dagger_1C_1=&\Gamma\begin{pmatrix}
    1&0\\
    0&0
  \end{pmatrix}\\
  C^\dagger_2C_2=&\Gamma\begin{pmatrix}
    0&0\\
    0&1
  \end{pmatrix}
}
Decay terms
\eqar{
  &\sum_m C_m\rho C^\dagger_m\\
  =&\begin{pmatrix}
    \Gamma\rho_{11}&0\\
    0&\Gamma\rho_{22}
  \end{pmatrix}\\
  &-\frac12\sum_m\paren{C^\dagger_m C_m\rho+\rho C^\dagger_m C_m}\\
  =&-\frac12\paren{C^\dagger_1 C_1\rho+\rho C^\dagger_1 C_1+C^\dagger_2 C_2\rho+\rho C^\dagger_2 C_2}
  \intertext{}
  =&-\frac\Gamma2\paren{\begin{pmatrix}
      1&0\\
      0&0
    \end{pmatrix}\rho+\rho\begin{pmatrix}
      1&0\\
      0&0
    \end{pmatrix}}-\frac\Gamma2\paren{\begin{pmatrix}
      0&0\\
      0&1
    \end{pmatrix}\rho+\rho\begin{pmatrix}
      0&0\\
      0&1
    \end{pmatrix}}\\
  =&-\begin{pmatrix}
    \Gamma\rho_{11}&\Gamma\rho_{12}\\
    \Gamma\rho_{21}&\Gamma\rho_{22}
  \end{pmatrix}
}
\eqar{
  \diff{\rho}{t}=&-\ui\sqr{H, \rho}+\begin{pmatrix}
    \Gamma\rho_{11}&0\\
    0&\Gamma\rho_{22}
  \end{pmatrix}-\begin{pmatrix}
    \Gamma\rho_{11}&\Gamma\rho_{12}\\
    \Gamma\rho_{21}&\Gamma\rho_{22}
  \end{pmatrix}\\
  =&\frac12\paren{\begin{pmatrix}
      0&-\Omega\\
      \Omega&0
    \end{pmatrix}\rho-\rho\begin{pmatrix}
      0&-\Omega\\
      \Omega&0
    \end{pmatrix}}-\begin{pmatrix}
    0&\Gamma\rho_{12}\\
    \Gamma\rho_{21}&0
  \end{pmatrix}\\
  =&\frac12\paren{\begin{pmatrix}
      \Omega\rho_{12}&-\Omega\rho_{11}\\
      \Omega\rho_{22}&-\Omega\rho_{21}
    \end{pmatrix}-\begin{pmatrix}
      -\Omega\rho_{21}&-\Omega\rho_{22}\\
      \Omega\rho_{11}&\Omega\rho_{12}
    \end{pmatrix}}-\begin{pmatrix}
    0&\Gamma\rho_{12}\\
    \Gamma\rho_{21}&0
  \end{pmatrix}\\
  =&\begin{pmatrix}
    \dfrac\Omega2\paren{\rho_{12}+\rho_{21}}&\dfrac\Omega2\paren{\rho_{22}-\rho_{11}}-\Gamma\rho_{12}\\
    \dfrac\Omega2\paren{\rho_{22}-\rho_{11}}-\Gamma\rho_{21}&-\dfrac\Omega2\paren{\rho_{12}+\rho_{21}}
  \end{pmatrix}
}
Let $x=\rho_{12}+\rho_{21}$, $y=\rho_{22}-\rho_{11}$
\eqar{
  \diff{x}{t}=&\Omega y-\Gamma x\\
  \diff{y}{t}=&-\Omega x\\
  \diff[2]{y}{t}=&-\Omega\diff{x}{t}\\
  =&-\Omega\paren{\Omega y-\Gamma x}\\
  =&-\Omega^2y+\Gamma\Omega x\\
  =&-\Omega^2y-\Gamma\diff{y}{t}\\
  0=&\diff[2]{y}{t}+\Gamma\diff{y}{t}+\Omega^2y
  \intertext{Assume underdamped ($4\Omega^2>\Gamma^2$). Let $\Omega'=\sqrt{4\Omega^2-\Gamma^2}/2$}
  y=&\exp\paren{-\frac{\Gamma t}{2}}\paren{c_1\sin\Omega't+c_2\cos\Omega't}
}
Initial condition
\eqar{
  x\paren{0}=&0\\
  y\paren{0}=&-1
}
So $c_2=-1$
\eqar{
  y=&\exp\paren{-\frac{\Gamma t}{2}}\paren{c_1\sin\Omega't-\cos\Omega't}\\
  \left.\diff{y}{t}\right|_{t=0}=&\frac{\Gamma}{2}+c_1\Omega'\\
  y=&-\exp\paren{-\frac{\Gamma t}{2}}\paren{\frac{\Gamma}{2\Omega'}\sin\Omega't+\cos\Omega't}\\
}

\section{State changing decay}
Jump operators
\eqar{
  C_1=&\sqrt{\Gamma}\begin{pmatrix}
    0&0\\
    1&0
  \end{pmatrix}\\
  C_2=&\sqrt{\Gamma}\begin{pmatrix}
    0&1\\
    0&0
  \end{pmatrix}\\
  C^\dagger_1=&\sqrt{\Gamma}\begin{pmatrix}
    0&1\\
    0&0
  \end{pmatrix}\\
  C^\dagger_2=&\sqrt{\Gamma}\begin{pmatrix}
    0&0\\
    1&0
  \end{pmatrix}\\
  C^\dagger_1C_1=&\Gamma\begin{pmatrix}
    1&0\\
    0&0
  \end{pmatrix}\\
  C^\dagger_2C_2=&\Gamma\begin{pmatrix}
    0&0\\
    0&1
  \end{pmatrix}
}
Decay terms
\eqar{
  &\sum_m C_m\rho C^\dagger_m\\
  =&\begin{pmatrix}
    \Gamma\rho_{22}&0\\
    0&\Gamma\rho_{11}
  \end{pmatrix}\\
  &-\frac12\sum_m\paren{C^\dagger_m C_m\rho+\rho C^\dagger_m C_m}\\
  =&-\frac12\paren{C^\dagger_1 C_1\rho+\rho C^\dagger_1 C_1+C^\dagger_2 C_2\rho+\rho C^\dagger_2 C_2}
  \intertext{}
  =&-\frac\Gamma2\paren{\begin{pmatrix}
      1&0\\
      0&0
    \end{pmatrix}\rho+\rho\begin{pmatrix}
      1&0\\
      0&0
    \end{pmatrix}}-\frac\Gamma2\paren{\begin{pmatrix}
      0&0\\
      0&1
    \end{pmatrix}\rho+\rho\begin{pmatrix}
      0&0\\
      0&1
    \end{pmatrix}}\\
  =&-\begin{pmatrix}
    \Gamma\rho_{11}&\Gamma\rho_{12}\\
    \Gamma\rho_{21}&\Gamma\rho_{22}
  \end{pmatrix}
}
\eqar{
  \diff{\rho}{t}=&-\ui\sqr{H, \rho}+\begin{pmatrix}
    \Gamma\rho_{22}&0\\
    0&\Gamma\rho_{11}
  \end{pmatrix}-\begin{pmatrix}
    \Gamma\rho_{11}&\Gamma\rho_{12}\\
    \Gamma\rho_{21}&\Gamma\rho_{22}
  \end{pmatrix}\\
  =&\frac12\paren{\begin{pmatrix}
      0&-\Omega\\
      \Omega&0
    \end{pmatrix}\rho-\rho\begin{pmatrix}
      0&-\Omega\\
      \Omega&0
    \end{pmatrix}}+\begin{pmatrix}
    \Gamma\paren{\rho_{22}-\rho_{11}}&-\Gamma\rho_{12}\\
    -\Gamma\rho_{21}&-\Gamma\paren{\rho_{22}-\rho_{11}}
  \end{pmatrix}\\
  =&\frac12\paren{\begin{pmatrix}
      \Omega\rho_{12}&-\Omega\rho_{11}\\
      \Omega\rho_{22}&-\Omega\rho_{21}
    \end{pmatrix}-\begin{pmatrix}
      -\Omega\rho_{21}&-\Omega\rho_{22}\\
      \Omega\rho_{11}&\Omega\rho_{12}
    \end{pmatrix}}+\begin{pmatrix}
    \Gamma\paren{\rho_{22}-\rho_{11}}&-\Gamma\rho_{12}\\
    -\Gamma\rho_{21}&-\Gamma\paren{\rho_{22}-\rho_{11}}
  \end{pmatrix}\\
  =&\begin{pmatrix}
    \dfrac\Omega2\paren{\rho_{12}+\rho_{21}}+\Gamma\paren{\rho_{22}-\rho_{11}}&\dfrac\Omega2\paren{\rho_{22}-\rho_{11}}-\Gamma\rho_{12}\\
    \dfrac\Omega2\paren{\rho_{22}-\rho_{11}}-\Gamma\rho_{21}&-\dfrac\Omega2\paren{\rho_{12}+\rho_{21}}-\Gamma\paren{\rho_{22}-\rho_{11}}
  \end{pmatrix}
}
Let $x=\rho_{12}+\rho_{21}$, $y=\rho_{22}-\rho_{11}$
\eqar{
  \diff{x}{t}=&\Omega y-\Gamma x\\
  \diff{y}{t}=&-\Omega x-2\Gamma y\\
  \Omega x=&-\diff{y}{t}-2\Gamma y\\
  \diff[2]{y}{t}=&-\Omega\diff{x}{t}-2\Gamma\diff{y}{t}\\
  =&-\Omega\paren{\Omega y-\Gamma x}-2\Gamma\diff{y}{t}\\
  =&-\Omega^2y+\Gamma\Omega x-2\Gamma\diff{y}{t}\\
  =&-\Omega^2y-\Gamma\paren{\diff{y}{t}+2\Gamma y}-2\Gamma\diff{y}{t}\\
  =&-3\Gamma\diff{y}{t}-\paren{\Omega^2+2\Gamma^2}y\\
  0=&\diff[2]{y}{t}+3\Gamma\diff{y}{t}+\paren{\Omega^2+2\Gamma^2}y
  \intertext{Assume underdamped ($4\Omega^2>\Gamma^2$). Let $\Omega'=\sqrt{4\Omega^2-\Gamma^2}/2$}
  y=&\exp\paren{-\frac{\Gamma t}{2}}\paren{c_1\sin\Omega't+c_2\cos\Omega't}
}
Initial condition
\eqar{
  x\paren{0}=&0\\
  y\paren{0}=&-1
}
So $c_2=-1$
\eqar{
  y=&\exp\paren{-\frac{\Gamma t}{2}}\paren{c_1\sin\Omega't-\cos\Omega't}\\
  \left.\diff{y}{t}\right|_{t=0}=&\frac{\Gamma}{2}+c_1\Omega'\\
  y=&-\exp\paren{-\frac{\Gamma t}{2}}\paren{\frac{\Gamma}{2\Omega'}\sin\Omega't+\cos\Omega't}\\
}


\end{document}
